moved around for faster filing

rules_src.v
@@ -1,4 +1,5 @@
-(*rules*)
+(*rules*) 
+From mathcomp Require Import ssreflect ssrfun ssrbool seq eqtype ssrnat.
 Require Import Tactics Sequence source subst_src (*SimpSub*).
 
 Require Import Defined.
@@ -49,3 +50,99 @@ Inductive of_m : context -> term -> term -> Type :=
     of_m G R (reftp_m T) ->
     of_m G (deref_m R) (comp_m T) 
 | of_m_triv: forall G, of_m G triv_m unittp_m.
+
+(*reduction*)
+
+Definition store := seq term.
+
+(*weak head? reduction*)
+Inductive val: term -> Prop :=
+(*| val_var {i} : val (var i) *) (*can assume terms are closed*)
+| val_z : val z_m
+| val_succ {n} : val n -> val (succ_m n)
+| val_lam {M} : val (lam_m M)
+| val_ap {M1 M2} : val M1 -> val M2 -> (forall M3, M1 <> lam_m M3) -> val (app_m M1 M2)
+| val_ret {M} : val M -> val (ret_m M)
+| val_bind {M1 M2} : val M1 ->
+                     (forall M3 M4, M1 <> ret_m M3 /\ M1 <> ref_m M3 /\ M1 <> deref_m M3 /\
+                               M1 <> asgn_m M3 M4) -> val (bind_m M1 M2) (*what if M1 is asgn but bind
+                                     can't make any steps because M1 is stuck
+                                     either ill typed or open, neutral term, dw*)
+| val_ref {M} : val M -> val (ref_m M)
+| val_deref {M} : val M -> val (deref_m M)
+| val_asgn_m {M1 M2} : val M1 -> val M2 -> val (asgn_m M1 M2)
+| val_triv : val triv_m
+| val_loc {i} : val (loc_m i).
+
+
+Definition asgn M i v := set_nth triv_m M i v.
+Definition get M i := nth triv_m M i.
+
+                          
+
+                
+(*weak head reduction
+ karl's reduce is nondeterministic*)
+Inductive reduce : (prod store term) -> (prod store term) -> Prop :=
+| reduce_ref {e M e' M'}: reduce (M, e) (M', e') ->
+  reduce (M, ref_m e) (M', ref_m e')
+| reduce_deref {e M e' M'}: reduce (M, e) (M', e') ->
+  reduce (M, deref_m e) (M', deref_m e')
+| reduce_asgn1 {e1 e2 M e1' M'}: reduce (M, e1) (M', e1') ->
+  reduce (M, asgn_m e1 e2) (M', asgn_m e1' e2)
+| reduce_asgn2 {v1 e2 M e2' M'}:
+    val v1 -> 
+    reduce (M, e2) (M', e2') ->
+    reduce (M, asgn_m v1 e2) (M', asgn_m v1 e2')
+| reduce_bind {e1 e2 M e1' M'}: reduce (M, e1) (M', e1') ->
+                                reduce (M, bind_m e1 e2) (M', bind_m e1' e2)
+| reduce_ret {e M e' M'}: reduce (M, e) (M', e') ->
+                          reduce (M, ret_m e) (M', ret_m e')
+| reduce_bindref {v e2 M} : val v ->
+                            reduce (M, bind_m (ref_m v) e2)
+                                   (rcons M v, subst1 e2 (loc_m (size M)))
+| reduce_bindasgn {l v e2 M} : val (asgn_m (loc_m l) v) ->
+                               reduce (M, bind_m (asgn_m (loc_m l) v) e2)
+                                      (asgn M l v, subst1 triv_m e2)
+| reduce_bindderef {l e2 M} : val (deref_m (loc_m l)) ->
+                              reduce (M, bind_m (deref_m (loc_m l)) e2)
+                                     (M, subst1 (get M l) e2)
+| reduce_nat {n n' M M'} : reduce (M, n) (M', n') ->
+                           reduce (M, succ_m n) (M', succ_m n')
+| reduce_app1 {f arg arg' M M'} : reduce (M, arg) (M', arg') ->
+                                  reduce (M, (app_m f arg)) (M', (app_m f arg'))
+| reduce_app2 {f f' v M M'} : val v ->
+                              reduce (M, f) (M', f') ->
+                              reduce (M, (app_m f v)) (M', (app_m f' v))
+
+| reduce_app_beta {v f M M'} :
+    val v ->
+    val f -> reduce (M, (app_m (lam_m f) v)) (M', (subst1 v f)).
+(*
+Inductive reduce : (prod store term) -> (prod store term) -> Prop :=
+| reduce_var {i M} : reduce (M, (var i)) (M, (var i))
+| reduce_ref {e M e' M'}: reduce (M, e) (M', e') ->
+  reduce (M, ref_m e) (M', ref_m e')
+| reduce_deref {e M e' M'}: reduce (M, e) (M', e') ->
+  reduce (M, deref_m e) (M', deref_m e')
+| reduce_asgn1 {e1 e2 M e1' M'}: reduce (M, e1) (M', e1') ->
+  reduce (M, asgn_m e1 e2) (M', asgn_m e1' e2)
+| reduce_asgn2 {v1 e2 M e2' M'}:
+    reduce (M, v1) (M, v1) -> (*v1 is value...kind of ruins normalization property of language?
+                              can't use thsi for v is a value cuz could do
+                              (asign v, e2) -> asgn(v, e2) by reduce_asgn1 even if e2
+                              is not a value*)
+    reduce (M, e2) (M', e2') ->
+    reduce (M, asgn_m v1 e2) (M', asgn_m v1 e2')
+| reduce_bind {e1 e2 M e1' M'}: reduce (M, e1) (M', e1') ->
+                                reduce (M, bind_m e1 e2) (M', bind_m e1' e2)
+| reduce_ret {e M e' M'}: reduce (M, e) (M', e') ->
+                          reduce (M, ret_m e) (M', ret_m e')
+| reduce_bindref {v e2 M} : reduce (M, v) (M, v) ->
+                            reduce (M, bind_m (ref_m v) e2)
+                                   (rcons M v, subst1 e2 (loc_m (size M)))
+                                   | reduce_bindas {l v e2 M} : reduce (M, asgn)
+| reduce_app_beta {n n' m M M'} :
+    reduce (M, n) (M', n')
+    -> reduce (M, (app_m (lam_m m) n)) (M', (subst1 n' m)).
+*)
