help0.v
@@ -1,0 +1,69 @@
+From Coq Require Import Lists.List.
+From mathcomp Require Import ssreflect ssrfun ssrbool seq eqtype ssrnat.
+From istari Require Import Tactics Sequence source subst_src rules_src.
+From istari Require Import basic_types0 Syntax Subst SimpSub Promote Hygiene
+     ContextHygiene Equivalence Rules Defined.
+
+(*small abbreviations that will help us later*)
+Definition app3 w i u l : term obj :=
+ app (app (app w i) u) l.
+
+(*quickly access the nth element of the big tuple in the comp type*)
+Definition picomp1 (M: term obj) := ppi1 M.
+Definition picomp2 (M: term obj) := ppi1 (ppi1 (ppi2 M) ). 
+Definition picomp3 (M: term obj) := ppi2 (ppi1 (ppi2 M)). 
+Definition picomp4 (M: term obj) := ppi2 (ppi2 M).
+(********************************************)
+(*useful types*)
+
+Definition plus L R : (term obj) := sigma booltp (bite (var 0) (subst (sh 1) L)
+                                           (subst (sh 1) R) ).
+Definition inl L: term obj := ppair btrue L.
+Definition inr R: term obj := ppair bfalse R.
+
+Definition opt w: term obj := sigma booltp (bite (var 0) w unittp).
+
+Definition laters A : term obj := rec (plus (shift 1 A) (fut (var 0))).
+(*notice similarity w type of nat in logic*)
+(********************************************)
+
+
+(*useful terms*)
+
+(*Unguarded recursion*)
+Definition Yc: (term obj) := lam ((*f := 0*)
+                   app
+                     (lam ( (*f := 1, x := 0*)
+                          let f := (var 1) in
+                          let x := (var 0) in
+                app f (next (app (prev x) x))
+                        )
+                     )
+                (next
+                   (lam (*f := 1, x := 0*)
+                      (
+                          let f := (var 1) in
+                          let x := (var 0) in
+                   app f (next (app (prev x) x))
+                      )
+                ))
+).
+Definition ret: term obj := lam (inl (var 0)).
+
+Definition ret_a x := inl x.
+
+Definition bind : term obj := app Yc
+   (lam   ( (*f := 0*)
+      lam ( (*f:= 1, x := 0*)
+          lam ( (*f:= 2, x := 1, g := 0*)
+              let f := (var 2) in
+              let x := (var 1) in
+              let g := (var 0) in
+              let y := ppi2 x in
+         bite (ppi1 x) (app g y)
+              (let y' := prev y in
+               let f' := prev f in
+               inr (next (app (app f' y') g))) )
+        ))).
+
+Definition make_bind E1 E2 := app (app bind E1) E2.
