simulation.v
@@ -1,0 +1,11 @@
+
+Require Import Program Equality Ring Lia Omega.
+From Coq Require Import ssreflect ssrfun ssrbool.
+From mathcomp Require Import seq eqtype ssrnat.
+From istari Require Import lemmas0
+     source subst_src rules_src basic_types0
+     help0 subst_help0.
+From istari Require Import Sigma Tactics
+     Syntax Subst SimpSub Promote Hygiene
+     ContextHygiene Equivalence Equivalences.
+From istari Require Import Rules Defined DefsEquiv.
