subst_help.v
@@ -1,62 +1,115 @@
+
 From Coq.Lists Require Import List.
 From mathcomp Require Import ssreflect ssrfun ssrbool seq eqtype ssrnat.
-From istari Require Import source subst_src rules_src help subst_help0.
+From istari Require Import source subst_src rules_src basic_types help.
 From istari Require Import Sigma Tactics
      Syntax Subst SimpSub Promote Hygiene
      ContextHygiene Equivalence Rules Defined.
 
+Lemma subst_world: forall s,
+    subst s world = world.
+intros. unfold world. unfold preworld. unfold nattp. auto. Qed.  
+Hint Rewrite subst_world: core subst1.
+
+Lemma subst_nat: forall s,
+    @ subst obj s nattp = nattp.
+  intros. unfold nattp. auto. Qed.
+
+Hint Rewrite subst_nat: core subst1.
+
+Lemma subst_pw: forall s,
+    subst s preworld = preworld.
+intros. unfold preworld. unfold nattp. auto. Qed.
+Hint Rewrite subst_pw : core subst1.
+
+Lemma subst_U0: forall s,
+    (@ subst obj s (univ nzero)) = univ nzero.
+  auto. Qed.
+Lemma subst_subseq: forall w1 w2 l1 l2 s,
+       (subst s
+              (subseq w1 l1 w2 l2)) = subseq (subst s w1)
+                                             (subst s l1)
+                                             (subst s w2)
+                                             (subst s l2).
+   intros. unfold subseq.
+   unfold app3.
+   simpsub_bigs.
+   auto.
+ Qed.
+
+Lemma subst_laters: forall s A, (subst s (laters A)) = (laters (subst s A)).
+  intros. unfold laters. unfold plus. rewrite subst_rec. rewrite subst_sigma.
+  rewrite subst_booltp. rewrite subst_bite. simpsub. simpl.
+  repeat rewrite <- subst_sh_shift. simpsub. auto. Qed.
+
+Lemma subst_store: forall w l s, subst s (store w l) = store (subst s w) (subst s l).
+  intros. unfold store. unfold gettype. simpsub_big. auto. Qed.
+
+Hint Rewrite subst_store: core subst1.
 
 
-Lemma size_substctx :
-  forall s G, size (@substctx obj s G) = size G.
-Proof.
-  intros. move: (length_substctx obj s G). apply.
+ Lemma subst_move: forall A l1 l2 s, (subst s (move A l1 l2)) = move A (subst s l1) (subst s l2).
+   intros. induction A; unfold make_subseq_trans;
+unfold leq_trans_fn_app; unfold leq_trans_fn; simpsub_big; simpl; auto.
+   { unfold make_subseq_trans;
+unfold leq_trans_fn_app; unfold leq_trans_fn; simpsub_big; simpl; auto.
+}
+   { unfold make_subseq_trans;
+unfold leq_trans_fn_app; unfold leq_trans_fn; simpsub_big; simpl; auto.
+}
+   { unfold make_subseq_trans;
+       unfold lt_trans_fn_app; unfold leq_trans_fn_app;
+         unfold leq_trans_fn; simpsub_big; simpl; auto.
+}
+ Qed.
+
+Hint Rewrite subst_move: core subst1.
+
+Lemma subst_moveapp s A l1 l2 m1 m2 : (subst s (move_app A l1 l2 m1 m2)) =
+                              move_app A (subst s l1) (subst s l2) (subst s m1) (subst s m2).
+   unfold move_app. simpsub_big. auto. Qed.
+
+Lemma subst_consb w l x s: @ subst obj s (cons_b w l x) =
+                           cons_b (subst s w) (subst s l) (subst s x).
+  unfold cons_b. simpsub_big. auto.
 Qed.
 
-Hint Rewrite size_substctx.
+Hint Rewrite subst_consb : subst1 core.
 
-Lemma substctx_app: forall G1 G2 s,
-    @substctx obj s (G1 ++ G2) = (substctx (under (size G2) s) G1) ++ (substctx s G2).
-  intros. induction G1; simpsub. repeat rewrite cat0s. auto.
-  simpl. simpsub. repeat rewrite plusE.
-  replace ((length G1) + (size G2)) with (size (G1 ++ G2)).
-  rewrite - IHG1. auto.
-  rewrite size_cat. auto. Qed.
+Lemma subst_make_subseq_trans: forall s a b c d e, (subst s (make_subseq_trans a b c d e)) = (make_subseq_trans
+                                                                                 (subst s a)
+                                                                                 (subst s b)
+                                                                                 (subst s c)
+                                                                                 (subst s d)
+                                                                                 (subst s e)
+                                                                                        ).
+  intros. unfold make_subseq_trans. unfold leq_trans_fn_app. unfold leq_trans_fn. simpsub. auto. Qed.
 
-Lemma substctx_rcons: forall G1 g s,
-    @substctx obj s (rcons G1 g) = rcons (substctx (under 1 s) G1) (substh s g).
-  intros. repeat rewrite - cats1. rewrite substctx_app. simpl. auto. Qed.
+Hint Rewrite subst_make_subseq_trans: core subst1.
+Hint Rewrite <- subst_make_subseq_trans : inv_subst.
 
+Lemma subst_lttp: forall s,
+    @ subst obj s (lttp) = lttp.
+  intros. unfold lttp.
+  simpsub. rewrite subst_leqtp. unfold nsucc. simpsub. simpl.
+  rewrite subst_leqtp. auto. Qed.
+Hint Rewrite subst_leqtp: core subst1.
 
-Lemma sh_sum :
-  forall m n t,
-    @subst obj (sh n) (subst (sh m) t) = @subst obj (sh (n+m)) t.
-  intros. repeat rewrite subst_sh_shift.
-  rewrite shift_sum. auto. Qed.
+Lemma subst_leq: forall s n1 n2,
+    @ subst obj s (leq_t n1 n2) =  leq_t (subst s n1) (subst s n2).
+  intros. unfold leq_t.  repeat rewrite subst_app. auto. 
+Qed.
 
+Lemma subst_lt: forall s n1 n2,
+    subst s (lt_t n1 n2) = lt_t (subst s n1) (@ subst obj s n2).
+  intros. repeat rewrite subst_app. rewrite subst_lttp. auto. Qed. 
 
-(*substitutions for moving variables around in context*)
-(*move old to new*)
-Fixpoint gen_sub_mvl G := match G with
-                        0 => id
-                          | n'.+1 =>
-@compose obj (under n' (dot (var 1) (dot (var 0) (sh 2)))) (gen_sub_mvl n')
-                                    end.
+Lemma subst_nth: forall s m1 m2, (subst s (nth m1 m2)) = (nth (subst s m1) (subst s m2)). intros. unfold nth. simpsub. auto. Qed.
 
-(*move new to old*)
-Fixpoint gen_sub_mvr E := match E with
-                        0 => id
-    | n'.+1 => @compose obj (gen_sub_mvr n')
-(under n' (dot (var 1) (dot (var 0) (sh 2))))
-                          end.
+Lemma subst_make_subseq: forall s, (subst s make_subseq) = make_subseq.
+  intros. unfold make_subseq. simpsub. auto. Qed.
 
-Fixpoint gen_sub_mvl_list g v :=
-  match v with
-    0 => id
-          | S v' => compose (gen_sub_mvl_list g v') (under v' (gen_sub_mvl g)) end.
-
-Fixpoint gen_sub_mvr_list g v :=
-  match v with
-    0 => id
-          | S v' => compose (under v' (gen_sub_mvr g )) (gen_sub_mvr_list g v') end.
-
+Hint Rewrite subst_subseq subst_leq subst_lttp subst_lt
+     subst_pw subst_world subst_nth subst_laters subst_make_subseq subst_ltb
+subst_moveapp
+.
