subst_help0.v
@@ -1,6 +1,6 @@
 From Coq.Lists Require Import List.
 From mathcomp Require Import ssreflect ssrfun ssrbool seq eqtype ssrnat.
-From istari Require Import source subst_src rules_src basic_types0 basic_types help.
+From istari Require Import source subst_src rules_src basic_types0 help0.
 From istari Require Import Sigma Tactics
      Syntax Subst SimpSub Promote Hygiene
      ContextHygiene Equivalence Rules Defined.
@@ -49,14 +49,6 @@ Ltac var_nf cap := var_nf_help cap 1.
 Lemma fold_subst1:  forall m1 m2, (@ subst obj (dot m1 id) m2) = subst1 m1 m2.
 intros. auto. Qed.
 
-Lemma subst_pw: forall s,
-    subst s preworld = preworld.
-intros. unfold preworld. unfold nattp. auto. Qed.
-Hint Rewrite subst_pw : core subst1.
-
-Lemma subst_U0: forall s,
-    (@ subst obj s (univ nzero)) = univ nzero.
-  auto. Qed.
 
 
 
@@ -70,16 +62,6 @@ Hint Rewrite subst_minus: core subst1. *)
 
 
 
-Lemma subst_world: forall s,
-    subst s world = world.
-intros. unfold world. unfold preworld. unfold nattp. auto. Qed.  
-Hint Rewrite subst_world: core subst1.
-
-Lemma subst_nat: forall s,
-    @ subst obj s nattp = nattp.
-  intros. unfold nattp. auto. Qed.
-
-Hint Rewrite subst_nat: core subst1.
 
 Lemma subst_nzero: forall s,
     @ subst obj s nzero = nzero.
@@ -92,34 +74,6 @@ Lemma subst_bind: forall s m1 m2,
   intros. auto. Qed.
 
 
-Lemma subst_lttp: forall s,
-    @ subst obj s (lttp) = lttp.
-  intros. unfold lttp.
-  simpsub. rewrite subst_leqtp. unfold nsucc. simpsub. simpl.
-  rewrite subst_leqtp. auto. Qed.
-Hint Rewrite subst_leqtp: core subst1.
-
-Lemma subst_leq: forall s n1 n2,
-    @ subst obj s (leq_t n1 n2) =  leq_t (subst s n1) (subst s n2).
-  intros. unfold leq_t.  repeat rewrite subst_app. auto. 
-Qed.
-
-Lemma subst_lt: forall s n1 n2,
-    subst s (lt_t n1 n2) = lt_t (subst s n1) (@ subst obj s n2).
-  intros. repeat rewrite subst_app. rewrite subst_lttp. auto. Qed. 
-
-Lemma subst_subseq: forall w1 w2 l1 l2 s,
-       (subst s
-              (subseq w1 l1 w2 l2)) = subseq (subst s w1)
-                                             (subst s l1)
-                                             (subst s w2)
-                                             (subst s l2).
-   intros. unfold subseq.
-   unfold app3.
-   simpsub_bigs.
-   auto.
- Qed.
-
 
 
 Lemma subst_ret: forall s, subst s ret = ret.
@@ -128,15 +82,7 @@ Lemma subst_ret: forall s, subst s ret = ret.
 Lemma subst_ret_a: forall s m, subst s (ret_a m) = ret_a (subst s m).
   intros. unfold ret_a. unfold ret. unfold inl. simpsub. auto. Qed.
 
-Lemma subst_laters: forall s A, (subst s (laters A)) = (laters (subst s A)).
-  intros. unfold laters. unfold plus. rewrite subst_rec. rewrite subst_sigma.
-  rewrite subst_booltp. rewrite subst_bite. simpsub. simpl.
-  repeat rewrite <- subst_sh_shift. simpsub. auto. Qed.
 
-Lemma subst_nth: forall s m1 m2, (subst s (nth m1 m2)) = (nth (subst s m1) (subst s m2)). intros. unfold nth. simpsub. auto. Qed.
-
-Lemma subst_make_subseq: forall s, (subst s make_subseq) = make_subseq.
-  intros. unfold make_subseq. simpsub. auto. Qed.
 
 Lemma subst_picomp1: forall s m, (subst s (picomp1 m)) = picomp1 (subst s m).
   intros. unfold picomp1. simpsub. auto. Qed.
@@ -150,47 +96,22 @@ Lemma subst_picomp3: forall s m, (subst s (picomp3 m)) = picomp3 (subst s m).
 Lemma subst_picomp4: forall s m, (subst s (picomp4 m)) = picomp4 (subst s m).
   intros. unfold picomp4. simpsub. auto. Qed.
 
-Hint Rewrite subst_U0 subst_ret subst_ret_a subst_subseq subst_leq subst_leq
-     subst_lttp subst_lt subst_nzero subst_nat subst_world subst_pw subst_world
-     subst_nth subst_laters subst_picomp1 subst_picomp2 subst_picomp4
-     subst_picomp3 subst_make_subseq subst_theta  subst_ltb: core subst1.
+Hint Rewrite subst_U0 subst_ret subst_ret_a
+     subst_nzero subst_nat 
+ subst_picomp1 subst_picomp2 subst_picomp4
+     subst_picomp3 subst_theta: core subst1.
 
 Hint Rewrite <- subst_sh_shift: core subst1.
 
 Hint Unfold subst1: subst1.
 
 
-Lemma subst_store: forall w l s, subst s (store w l) = store (subst s w) (subst s l).
-  intros. unfold store. unfold gettype. simpsub_big. auto. Qed.
-
-Hint Rewrite subst_store: core subst1.
 
 
 Lemma subst_nsucc s n : (subst s (nsucc n)) = @ nsucc obj (subst s n).
   unfold nsucc. simpsub. auto. Qed.
 
- Lemma subst_move: forall A l1 l2 s, (subst s (move A l1 l2)) = move A (subst s l1) (subst s l2).
-   intros. induction A; unfold make_subseq_trans;
-unfold leq_trans_fn_app; unfold leq_trans_fn; simpsub_big; simpl; auto.
-   { unfold make_subseq_trans;
-unfold leq_trans_fn_app; unfold leq_trans_fn; simpsub_big; simpl; auto.
-}
-   { unfold make_subseq_trans;
-unfold leq_trans_fn_app; unfold leq_trans_fn; simpsub_big; simpl; auto.
-}
-   { unfold make_subseq_trans;
-       unfold lt_trans_fn_app; unfold leq_trans_fn_app;
-         unfold leq_trans_fn; simpsub_big; simpl; auto.
-}
- Qed.
-
-Hint Rewrite subst_move: core subst1.
-
-Lemma subst_moveapp s A l1 l2 m1 m2 : (subst s (move_app A l1 l2 m1 m2)) =
-                              move_app A (subst s l1) (subst s l2) (subst s m1) (subst s m2).
-   unfold move_app. simpsub_big. auto. Qed.
-
-Hint Rewrite subst_nsucc subst_moveapp: core subst1.
+Hint Rewrite subst_nsucc : core subst1.
 
 
 Lemma subst_inr: forall s t, subst s (inr t)  = inr (subst s t).
@@ -205,21 +126,3 @@ Lemma subst_plus: forall s A B, subst s (plus A B) =
   Qed.
   Hint Rewrite subst_inl subst_inr subst_plus: core subst1.
 
-Lemma subst_consb w l x s: @ subst obj s (cons_b w l x) =
-                           cons_b (subst s w) (subst s l) (subst s x).
-  unfold cons_b. simpsub_big. auto.
-Qed.
-
-Hint Rewrite subst_consb : subst1 core.
-
-Lemma subst_make_subseq_trans: forall s a b c d e, (subst s (make_subseq_trans a b c d e)) = (make_subseq_trans
-                                                                                 (subst s a)
-                                                                                 (subst s b)
-                                                                                 (subst s c)
-                                                                                 (subst s d)
-                                                                                 (subst s e)
-                                                                                        ).
-  intros. unfold make_subseq_trans. unfold leq_trans_fn_app. unfold leq_trans_fn. simpsub. auto. Qed.
-
-Hint Rewrite subst_make_subseq_trans: core subst1.
-Hint Rewrite <- subst_make_subseq_trans : inv_subst.
